new-backend/bvl_to_bvpScript.sml
@@ -2,7 +2,7 @@ open HolKernel Parse boolLib bossLib; val _ = new_theory "bvl_to_bvp";
 
 open pred_setTheory arithmeticTheory pairTheory listTheory combinTheory;
 open finite_mapTheory sumTheory relationTheory stringTheory optionTheory;
-open bytecodeTheory bytecodeEvalTheory bvlTheory;
+open bytecodeTheory bvlTheory;
 open bvl_inlineTheory bvpTheory;
 
 infix \\ val op \\ = op THEN;
@@ -14,42 +14,52 @@ val index_of_def = Define `
   (index_of n (x::xs) = if x = n then 0 else 1 + index_of n xs)`;
 
 val bComp_def = tDefine "bComp" `
-  (bComp (n:num) (env:num list) [] = (Skip,[]:num list,n)) /\
-  (bComp n env (x::y::xs) =
-     let (c1,v1,n1) = bComp n env [x] in
-     let (c2,vs,n2) = bComp n1 env (y::xs) in
+  (bComp (n:num) (env:num list) tail [] =
+    (Skip,[]:num list,n)) /\
+  (bComp n env tail (x::y::xs) =
+     let (c1,v1,n1) = bComp n env F [x] in
+     let (c2,vs,n2) = bComp n1 env F (y::xs) in
        (Seq c1 c2, HD v1 :: vs, n2)) /\
-  (bComp n env [Var v] =
-    (Move n (index_of v env), [n], n+1)) /\
-  (bComp n env [If x1 x2 x3] =
-     let (c1,v1,n1) = bComp n env [x1] in
-     let (c2,v2,n2) = bComp n1 env [x2] in
-     let (c3,v3,n3) = bComp n2 env [x3] in
-       (If [Prog c1; Assert (HD v1) T]
-          (Seq c2 (Move n3 (HD v2)))
-          (Seq c2 (Move n3 (HD v3))),
-        [n3],n3+1)) /\
-  (bComp n env [Let xs x2] =
-     let (c1,vs,n1) = bComp n env xs in
-     let (c2,v2,n2) = bComp n1 vs [x2] in
+  (bComp n env tail [Var v] =
+     if tail
+     then (Return (index_of v env), [n], n+1)
+     else (Move n (index_of v env), [n], n+1)) /\
+  (bComp n env tail [If x1 x2 x3] =
+     let (c1,v1,n1) = bComp n env F [x1] in
+     let (c2,v2,n2) = bComp n1 env tail [x2] in
+     let (c3,v3,n3) = bComp n2 env tail [x3] in
+       if tail then
+         (If [Prog c1; Assert (HD v1) T] c2 c3,[n3],n3+1)
+       else
+         (If [Prog c1; Assert (HD v1) T]
+            (Seq c2 (Move n3 (HD v2)))
+            (Seq c3 (Move n3 (HD v3))),
+          [n3],n3+1)) /\
+  (bComp n env tail [Let xs x2] =
+     let (c1,vs,n1) = bComp n env F xs in
+     let (c2,v2,n2) = bComp n1 vs tail [x2] in
        (Seq c1 c2, v2, n2)) /\
-  (bComp n env [Raise x1] =
-     let (c1,v1,n1) = bComp n env [x1] in
+  (bComp n env tail [Raise x1] =
+     let (c1,v1,n1) = bComp n env F [x1] in
        (Seq c1 (Raise (HD v1)), v1, n1)) /\
-  (bComp n env [Handle x1 x2] =
-     let (c1,v1,n1) = bComp n env [x1] in
-     let (c2,v2,n2) = bComp (n1+1) env [x2] in
-       (Handle (Seq c1 (Move n2 (HD v1))) n2 n1
-               (Seq c2 (Move n2 (HD v2))), [n2], n2+1)) /\
-  (bComp n env [Op op xs] =
-     let (c1,vs,n1) = bComp n env xs in
-       (Seq c1 (Assign n1 op vs), [n1], n1+1)) /\
-  (bComp n env [Tick x1] =
-     let (c1,v1,n1) = bComp n env [x1] in
-       (Seq Tick c1, v1, n1)) /\
-  (bComp n env [Call dest xs] =
-     let (c1,vs,n1) = bComp n env xs in
-       (Seq c1 (Call n1 dest vs), [n1], n+1))`
- (WF_REL_TAC `measure (bvl_exp1_size o SND o SND)`);
+  (bComp n env tail [Handle x1 x2] =
+     let (c1,v1,n1) = bComp n env F [x1] in
+     let (c2,v2,n2) = bComp (n1+1) env F [x2] in
+     let c3 = Handle (Seq c1 (Move n2 (HD v1))) n2 n1
+                     (Seq c2 (Move n2 (HD v2))) in
+       (if tail then Seq c3 (Return n2) else c3, [n2], n2+1)) /\
+  (bComp n env tail [Op op xs] =
+     let (c1,vs,n1) = bComp n env F xs in
+     let c2 = Seq c1 (Assign n1 op vs) in
+       (if tail then Seq c2 (Return n1) else c2, [n1], n1+1)) /\
+  (bComp n env tail [Tick x1] =
+     let (c1,v1,n1) = bComp n env F [x1] in
+     let c2 = Seq Tick c1 in
+       (if tail then Seq c2 (Return n1) else c2, v1, n1)) /\
+  (bComp n env tail [Call dest xs] =
+     let (c1,vs,n1) = bComp n env F xs in
+     let ret = (if tail then NONE else SOME n1) in
+       (Seq c1 (Call ret dest vs), [n1], n+1))`
+ (WF_REL_TAC `measure (bvl_exp1_size o SND o SND o SND)`);
 
 val _ = export_theory();
